[Cohen1993, Lemma 5.4.5] Let $$I_1=a_1\Z+\frac{-b_1+\sqrt{\Delta}}{2}\Z$$ be an ideal of $$\mathcal{O}_\Delta$$, and let $$I_2$$ be a similar ideal. Set $$s=(b_1+b_2)/2$$, $$n=(b_1-b_2)/2$$, $$d=\mathrm{gcd}(a_1, a_2, s)$$, and let $$u, v, w$$ be integers such that $$ua_1+va_2+ws=d$$. Then we have
$$
I_1\cdot I_2=d\left(A\Z+\frac{-B+\sqrt{\Delta}}{2}\right),
$$
where
$$
A=d_0\frac{a_1a_2}{d^2},\;
B=b_2+\frac{2a_2}{d}\left(v(s-b_2)-wc_2\right).
$$
In general, $$d_0=\mathrm{gcd}(a_1, a_2, s, c_1, c_2, n)$$. If at least one of the form $$(a_1, b_1, c_1)$$ or $$(a_2, b_2, c_2)$$ is primitive, then $$d_0=1$$.

<u>Proof.</u> The ideal $$I_3=I_1\cdot I_2$$ is generated as a $$\Z$$-module by the four products of the generators of $$I_1$$ and $$I_2$$. To be more specific, the four generators of $$I_3$$ are
$$
\begin{align}
g_1&=a_1a_2,\\
g_2&=-a_1b_2/2+(a_1/2)\sqrt{\Delta},\\
g_3&=-a_2b_1/2+(a_2/2)\sqrt{\Delta},\\
g_4&=(b_1b_2+\Delta)/4-(s/2)\sqrt{\Delta}.
\end{align}\label{gen}\tag{gen}
$$
Now by Proposition 5.2.1 we know that we can write
$$
I_3=C\left(A\Z+\frac{-B+\sqrt{\Delta}}{2}\right)
$$
for some integers $$A, B$$ and $$C$$. It is clear that $$C$$ is the smallest positive coefficient of $$\sqrt{\Delta}/2$$ in $$\eqref{gen}$$. So $$C=\mathrm{gcd}(a_1,a_2,s)$$ as stated.

Now we determine the value of $$AC$$, which is the least positive integer belonging to $$I_3$$. Any element of $$I_3$$ is of the form $$x=x_1g_1+x_2g_2+x_3g_3+x_4g_4$$ for integer $$x_i$$-s. The set $$I_3\cap \Z$$ is the set of such element with $$x_2a_1+x_3a_2-x_4s=0$$.

Using [Cohen1993, Exercise 5.11], the general solution to this equation is
$$
\begin{align}
x_1 &= \lambda_4,\\
x_2 &= \lambda_3\frac{a_2}{\gcd(a_1, a_2)}-\lambda_2\frac{-s}{\gcd(a_1,s)},\\
x_3 &= \lambda_1\frac{-s}{\gcd(a_2,s)}-\lambda_3\frac{a_1}{\gcd(a_1,a_2)},\\
x_4 &= \lambda_2\frac{a_1}{\gcd(a_1,s)}-\lambda_1\frac{a_2}{\gcd(a_2,s)}.
\end{align} \tag{xs}\label{xs}
$$
for arbitrary integers $$\lambda_i$$.

(ç¬”è®°1) æ–¹ç¨‹ $$u_2a_1+u_3a_2-u_4s=0$$ çš„æ„æ€æ˜¯ "ä»¤ $$\sqrt{\Delta}$$ é¡¹çš„ç³»æ•°ä¸º0". è¿™åœ¨é€»è¾‘ä¸Šæ˜¯ $$I_3$$ ä¸­çš„å…ƒç´ ä¸ºæ•´æ•°çš„å¿…è¦æ¡ä»¶. è¿˜éœ€æ’é™¤å…ƒç´ çš„æœ‰ç†éƒ¨åˆ†ä¸ºåŠæ•´æ•°çš„æƒ…å†µ. æœ‰ç†éƒ¨åˆ†è¡¨ç¤ºä¸º
$$
R_x=(a_1a_2)x_1+(-a_1b_2/2)x_2+(-a_2b_1/2)x_3
+\left(\left(b_1b_2+\Delta\right)/4\right)x_4. \tag{cal}\label{cal}
$$
æ ¹æ® $$\Delta=b^2-4ac$$ å¯çŸ¥ $$\Delta$$ ä¸ $$b$$ å¥‡å¶æ€§ç›¸åŒ. å½“ $$\Delta\equiv 0\pmod 4$$  æ—¶, $$b_1, b_2$$ éƒ½æ˜¯å¶æ•°, è¡¨è¾¾å¼ $$\eqref{cal}$$ çš„ç»“æœæ˜¯æ•´æ•°. è¿˜éœ€è€ƒå¯Ÿ $$\Delta\equiv 1 \pmod 4$$ çš„æƒ…å†µ. (ç¬”è®°1ç»“æŸ)

After a short calculation, we see that $$I_3\cap \Z=e\Z$$ where
$$
\begin{align}
t &=\gcd\left(
\frac{a_1a_2c_1}{\gcd(a_2,s)},
\frac{a_1a_2c_2}{\gcd(a_1,s)},
\frac{a_1a_2n}{\gcd(a_1,a_2)},
a_1a_2 \right) \\
&=\frac{a_1a_2}{\gcd(a_1, a_2, s)}
\gcd(a_1, a_2,s,c_1,c_2,n).
\end{align}
\tag{stride}\label{stride}
$$
This gives the claimed value $$A=d_0\frac{a_1a_2}{d^2}$$.

(ç¬”è®°2) è¿™short calculationéƒ½ç®—äº†ä»€ä¹ˆ? é¦–å…ˆå°† $$\eqref{xs}$$ ä»£å…¥ $$\eqref{cal}$$, å¾—åˆ°
$$
\begin{align}
R_x &=\frac{a_1a_2c_1}{\gcd(a_2,s)}\lambda_1-\frac{a_1a_2c_2}{\gcd(a_1,s)}\lambda_2+\frac{a_1a_2n}{\gcd(a_1,a_2)}\lambda_3 + a_1a_2\lambda_4.
\end{align} \tag{x.r}\label{x.r}
$$
æ˜¾ç„¶, ç›¸åŠ çš„å„é¡¹éƒ½æ˜¯æ•´æ•°, å› æ­¤ $$R_x$$ ä¹Ÿæ˜¯æ•´æ•°. æ ¹æ®ç†æƒ³çš„å®šä¹‰(åŠ æ³•ç¾¤, ä¹˜æ³•å°é—­), ä¸¤ä¸ªç†æƒ³çš„äº¤é›†æ˜¯è¿™ä¸¤ä¸ªç†æƒ³çš„ç†æƒ³. æ‰€ä»¥äº¤é›†ä¸€å®šæ˜¯ $$t\Z$$ çš„å½¢å¼. å› æ­¤, æ— è®ºè‡ªç”±æ•´æ•° $$\lambda_i$$ å–ä½•å€¼, $$R_x$$ éƒ½å°†å‘ˆç°å‡ºå‘¨æœŸæ€§, å‘¨æœŸä¸º $$\lambda_i$$ çš„å„ç³»æ•°çš„GCD. å…¬å¼$$\eqref{stride}$$ å°±æ˜¯è¿™ä¹ˆæ¥çš„. (ç¬”è®°2ç»“æŸ)

(ç¬”è®°3) å…¬å¼ $$\eqref{x.r}$$ ä¸­, $$\lambda_i$$ çš„å„ç³»æ•°æ˜¯æ€ä¹ˆç®—çš„?

$$\lambda_4$$ çš„ç³»æ•°æ˜¯æ˜¾ç„¶çš„, è¿™é‡Œç•¥è¿‡.

$$\lambda_3$$ çš„ç³»æ•°çš„æ¥å†å¦‚ä¸‹.
$$
a_1a_2n=-a_2a_1b_2/2+a_1a_2b_1/2.
$$
$$\lambda_2$$ çš„ç³»æ•°çš„æ¥å†å¦‚ä¸‹.
$$
\begin{align}
-a_1a_2c_2
&=-a_1b_2s/2+a_1(b_1b_2+\Delta)/4 \\
&=a_1(-b_1b_2-b_2^2+b_1b_2+\Delta)/4 \\
&=a_1(-b_1b_2-b_2^2+b_1b_2+b_2^2-4a_2c_2)/4.
\end{align}
$$
ç±»ä¼¼åœ°, $$\lambda_1$$ çš„ç³»æ•°çš„æ¥å†å¦‚ä¸‹.
$$
\begin{align}
a_1a_2c_1
&= a_2b_1s/2-a_2(b_1b_2+\Delta)/4 \\
&=a_2(b_1b_2+b_1^2-b_1b_2-b_1^2+4a_1c_1)/4.
\end{align}
$$
(ç¬”è®°3ç»“æŸ)

Finally, if $$d=ua_1+va_2+ws$$, one possible value of B is clearly
$$
\begin{align}
B
&= \frac{ua_1b_2+va_2b+1+w(b_1b_2+\Delta)/2}{d} \\
&= \frac{db_2+va_2(b_1-b_2)-2a_2c_2w}{d},
\end{align}
$$
thus proving the lemma. ğŸŸ©

[Cohen1993, Algorithm 5.4.9] (NUCOMP) Given two quadratic forms $$f_1=(a_1,b_1,c_1)$$ and $$f_2=(a_2,b_2,c_2)$$, which are primitive positive definite with the same discriminant. This algorithm computes the **composite** $$f_3=(a_3, b_3, c_3)$$ of $$f_1$$ and $$f_2$$. We assume the constant $$L=\lfloor\left(D/4\right)^{1/4}\rfloor$$ is already pre-computed.

